# Electromagnetismo II
## Problema T10-01

Demostrar que

```math
\int_0^a \sin\left(\frac{n\pi y}{a}\right)\sin\left(\frac{n'\pi y}{a}\right) dy
=
\begin{cases}
0           & \text{si } n' \neq n \\
\frac{a}{2} & \text{si } n' = n
\end{cases}
```

***Nota:*** $`n`$ y $`n'`$ son enteros.

---

**Solución**

Para escribir menos tomaré $`m = n \pi a`$ y $`m' = n' \pi a`$. Ahora supongamos que $`m = m'`$. Entonces

```math
\begin{align}
\int_0^a\sin(m y) \sin(m' y) dy
&= \int_0^a \left(\frac{1}{2} + \frac{1}{2}\cos(2m y)\right)dy \\
&= \left.\frac{1}{2}y + \frac{1}{4m}\sin(2m y)\right|_0^a \\
&= \left.\frac{1}{2}y + \frac{1}{4m}\sin(2n\pi y / a)\right|_0^a \\
&= \frac{a}{2}
```

En cambio para $`m \neq m'`$

```math
\begin{align}
\int_0^a\sin(m y) \sin(m' y) dy
&=  \int_0^a \frac{\cos[(m - m') y] - \cos[(m + m')y]}{2} dy \\
&=  \left. \frac{\sin[(m - m') y]}{2 (m - m')} - \frac{\sin[(m + m')y]}{2(m + m')} \right|_0^a  \\
&=  \frac{\sin[(m - m') a]}{2 (m - m')} - \frac{\sin[(m + m')a]}{2(m + m')}  \\
&=  \frac{\sin[(n - n')\pi]}{2 (m - m')} - \frac{\sin[(n + n')\pi]}{2(m + m')}  \\
&= 0
\end{align}
```
